platform/Xml.v
@@ -1,0 +1,18 @@
+Require Import XmlLang.
+Export XmlLang.
+
+
+Coercion XmlLang.Cdata : string >-> XmlLang.pat.
+Infix "/" := XmlLang.Tag : pat_scope.
+Infix "&" := XmlLang.Both (at level 41, right associativity) : pat_scope.
+Delimit Scope pat_scope with pat.
+
+Coercion XmlOutput.Cdata : string >-> XmlOutput.xml.
+Definition xcons (x : XmlOutput.xml) (xs : list XmlOutput.xml) : list XmlOutput.xml := x :: xs.
+Notation "<*> tag </> x1 , .. , xN </>" := (XmlOutput.Tag tag (xcons x1 .. (xcons xN nil) ..))
+  (tag at level 0) : out_scope.
+Delimit Scope out_scope with out.
+
+Notation "'Match' p 'Do' o 'end'" := {| Pattern := p%pat; Output := o%out |}.
+
+Ltac wf := repeat split; simpl; intuition congruence.
